Packet_Set.thy
@@ -116,6 +116,30 @@ subsection{*The set of all accepted packets*}
   using collect_allow_complete[where P=UNIV] by fast
 
 
+  text{*the complement of the allowed packets*}
+  fun collect_allow_compl :: "('a, 'p) match_tac \<Rightarrow> 'a rule list \<Rightarrow> 'p set \<Rightarrow> 'p set" where
+    "collect_allow_compl _ [] P = UNIV" |
+    "collect_allow_compl \<gamma> ((Rule m Accept)#rs) P = (P \<union> {p. \<not>matches \<gamma> m Accept p}) \<inter> (collect_allow_compl \<gamma> rs (P \<union> {p. matches \<gamma> m Accept p}))" |
+    "collect_allow_compl \<gamma> ((Rule m Drop)#rs) P = (collect_allow_compl \<gamma> rs (P \<union> {p. matches \<gamma> m Drop p}))"
+  
+  lemma collect_allow_compl_correct: "simple_ruleset rs \<Longrightarrow> (- collect_allow_compl \<gamma> rs ( - P)) = collect_allow \<gamma> rs P"
+    proof(induction \<gamma> rs P arbitrary: P rule: collect_allow.induct)
+    case 1 thus ?case by simp
+    next
+    case (2 \<gamma> r rs)
+      have set_simp1: "- {p \<in> P. \<not> matches \<gamma> r Accept p} = - P \<union> {p. matches \<gamma> r Accept p}" by blast
+      from 2 have IH: "\<And>P. - collect_allow_compl \<gamma> rs (- P) = collect_allow \<gamma> rs P" using simple_ruleset_tail by blast
+      from IH[where P="{p \<in> P. \<not> matches \<gamma> r Accept p}"] set_simp1 have
+        "- collect_allow_compl \<gamma> rs (- P \<union> Collect (matches \<gamma> r Accept)) = collect_allow \<gamma> rs {p \<in> P. \<not> matches \<gamma> r Accept p}" by simp
+      thus ?case by auto
+    next
+    case (3 \<gamma> r rs)
+      have set_simp1: "- {p \<in> P. \<not> matches \<gamma> r Drop p} = - P \<union> {p. matches \<gamma> r Drop p}" by blast
+      from 3 have IH: "\<And>P. - collect_allow_compl \<gamma> rs (- P) = collect_allow \<gamma> rs P" using simple_ruleset_tail by blast
+      from IH[where P="{p \<in> P. \<not> matches \<gamma> r Drop p}"] set_simp1 have
+        "- collect_allow_compl \<gamma> rs (- P \<union> Collect (matches \<gamma> r Drop)) = collect_allow \<gamma> rs {p \<in> P. \<not> matches \<gamma> r Drop p}" by simp
+      thus ?case by auto
+    qed(simp_all add: simple_ruleset_def)
 
 subsection{*The set of all dropped packets*}
   text{*
@@ -205,7 +229,30 @@ subsection{*The set of all dropped packets*}
   using collect_deny_sound[where P=UNIV] apply fast
   using collect_deny_complete[where P=UNIV] by fast
   
-
+  text{*the complement of the denied packets*}
+  fun collect_deny_compl :: "('a, 'p) match_tac \<Rightarrow> 'a rule list \<Rightarrow> 'p set \<Rightarrow> 'p set" where
+    "collect_deny_compl _ [] P = UNIV" |
+    "collect_deny_compl \<gamma> ((Rule m Drop)#rs) P = (P \<union> {p. \<not>matches \<gamma> m Drop p}) \<inter> (collect_deny_compl \<gamma> rs (P \<union> {p. matches \<gamma> m Drop p}))" |
+    "collect_deny_compl \<gamma> ((Rule m Accept)#rs) P = (collect_deny_compl \<gamma> rs (P \<union> {p. matches \<gamma> m Accept p}))"
+  
+  lemma collect_deny_compl_correct: "simple_ruleset rs \<Longrightarrow> (- collect_deny_compl \<gamma> rs ( - P)) = collect_deny \<gamma> rs P"
+    proof(induction \<gamma> rs P arbitrary: P rule: collect_deny.induct)
+    case 1 thus ?case by simp
+    next
+    case (3 \<gamma> r rs)
+      have set_simp1: "- {p \<in> P. \<not> matches \<gamma> r Accept p} = - P \<union> {p. matches \<gamma> r Accept p}" by blast
+      from 3 have IH: "\<And>P. - collect_deny_compl \<gamma> rs (- P) = collect_deny \<gamma> rs P" using simple_ruleset_tail by blast
+      from IH[where P="{p \<in> P. \<not> matches \<gamma> r Accept p}"] set_simp1 have
+        "- collect_deny_compl \<gamma> rs (- P \<union> Collect (matches \<gamma> r Accept)) = collect_deny \<gamma> rs {p \<in> P. \<not> matches \<gamma> r Accept p}" by simp
+      thus ?case by auto
+    next
+    case (2 \<gamma> r rs)
+      have set_simp1: "- {p \<in> P. \<not> matches \<gamma> r Drop p} = - P \<union> {p. matches \<gamma> r Drop p}" by blast
+      from 3 have IH: "\<And>P. - collect_deny_compl \<gamma> rs (- P) = collect_deny \<gamma> rs P" using simple_ruleset_tail by blast
+      from IH[where P="{p \<in> P. \<not> matches \<gamma> r Drop p}"] set_simp1 have
+        "- collect_deny_compl \<gamma> rs (- P \<union> Collect (matches \<gamma> r Drop)) = collect_deny \<gamma> rs {p \<in> P. \<not> matches \<gamma> r Drop p}" by simp
+      thus ?case by auto
+    qed(simp_all add: simple_ruleset_def)
 
 subsection{*Rulesets with default rules*}
   definition has_default :: "'a rule list \<Rightarrow> bool" where
@@ -224,6 +271,19 @@ subsection{*Rulesets with default rules*}
   apply(case_tac a)
          apply(auto simp: good_ruleset_def)
   done
+
+
+  lemma allow_set_by_collect_deny_compl: assumes "simple_ruleset rs" and "has_default rs"
+   shows "collect_deny_compl \<gamma> rs {} = {p. approximating_bigstep_fun \<gamma> p rs Undecided = Decision FinalAllow}"
+  proof -
+    from assms have univ: "{p. approximating_bigstep_fun \<gamma> p rs Undecided = Decision FinalAllow} \<union> {p. approximating_bigstep_fun \<gamma> p rs Undecided = Decision FinalDeny} = UNIV"
+    using simple_imp_good_ruleset has_default_UNIV by fast
+    from assms(1) collect_deny_compl_correct[where P=UNIV] have "collect_deny_compl \<gamma> rs {} = - collect_deny \<gamma> rs UNIV" by fastforce
+    moreover with collect_deny_sound_complete assms(1) have "\<dots> =  - {p. approximating_bigstep_fun \<gamma> p rs Undecided = Decision FinalDeny}" by fast
+    ultimately show ?thesis using univ by fastforce
+  qed
+  
+
 
 subsection{*Executable Packet Set Representation*}
 
@@ -648,6 +708,7 @@ lemma set_helper1:
   "- {p. matches \<gamma> m a p} =  {p. \<not> matches \<gamma> m a p}"
 by blast+
 
+(*
 fun collect_allow_compl_v1 :: "('a, 'p) match_tac \<Rightarrow> 'a rule list \<Rightarrow> 'p set \<Rightarrow> 'p set" where
   "collect_allow_compl_v1 _ [] P = {}" |
   "collect_allow_compl_v1 \<gamma> ((Rule m Accept)#rs) P = {p \<in> - P. matches \<gamma> m Accept p} \<union> (collect_allow_compl_v1 \<gamma> rs (P \<union> {p. matches \<gamma> m Accept p}))" |
@@ -677,19 +738,19 @@ apply(simp_all add: simple_ruleset_def)[6]
 apply(simp_all add: simple_ruleset_tail)
 apply(simp_all add: set_helper1(3) set_helper1(2)[simplified])
 done
+*)
 
 
-fun collect_allow_compl_v2_impl :: "'a rule list \<Rightarrow> 'a packet_set \<Rightarrow> 'a packet_set" where
-  "collect_allow_compl_v2_impl [] P = packet_set_UNIV" |
-  "collect_allow_compl_v2_impl ((Rule m Accept)#rs) P = packet_set_intersect 
-      (packet_set_union P  (packet_set_not (to_packet_set Accept m))) (collect_allow_compl_v2_impl rs (packet_set_opt (packet_set_union P (to_packet_set Accept m))))" |
-  "collect_allow_compl_v2_impl ((Rule m Drop)#rs) P = (collect_allow_compl_v2_impl rs (packet_set_opt (packet_set_union P (to_packet_set Drop m))))"
+fun collect_allow_compl_impl :: "'a rule list \<Rightarrow> 'a packet_set \<Rightarrow> 'a packet_set" where
+  "collect_allow_compl_impl [] P = packet_set_UNIV" |
+  "collect_allow_compl_impl ((Rule m Accept)#rs) P = packet_set_intersect 
+      (packet_set_union P  (packet_set_not (to_packet_set Accept m))) (collect_allow_compl_impl rs (packet_set_opt (packet_set_union P (to_packet_set Accept m))))" |
+  "collect_allow_compl_impl ((Rule m Drop)#rs) P = (collect_allow_compl_impl rs (packet_set_opt (packet_set_union P (to_packet_set Drop m))))"
 
 
-lemma collect_allow_compl_v2_impl: "simple_ruleset rs \<Longrightarrow> 
-  packet_set_to_set \<gamma> (collect_allow_compl_v2_impl rs P) = - collect_allow \<gamma> rs (- packet_set_to_set \<gamma>  P)"
-apply(simp add: collect_allow_compl_v1_correct[symmetric] )
-apply(simp add: collect_allow_compl_v2_correct)
+lemma collect_allow_compl_impl: "simple_ruleset rs \<Longrightarrow> 
+  packet_set_to_set \<gamma> (collect_allow_compl_impl rs P) = - collect_allow \<gamma> rs (- packet_set_to_set \<gamma>  P)"
+apply(simp add: collect_allow_compl_correct[symmetric] )
 apply(induction rs P arbitrary: P rule: collect_allow_impl_v1.induct)
 apply(simp_all add: simple_ruleset_def packet_set_union_correct packet_set_opt_correct packet_set_intersect_intersect packet_set_not_correct
     to_packet_set_set set_helper1 packet_set_UNIV )
@@ -697,27 +758,27 @@ done
 
 
 text{*take @{text "UNIV"} setminus the intersect over the result and get the set of allowed packets*}
-fun collect_allow_compl_v2_impl_tailrec :: "'a rule list \<Rightarrow> 'a packet_set \<Rightarrow> 'a packet_set list \<Rightarrow> 'a packet_set list" where
-  "collect_allow_compl_v2_impl_tailrec [] P PAs = PAs" |
-  "collect_allow_compl_v2_impl_tailrec ((Rule m Accept)#rs) P PAs =
-     collect_allow_compl_v2_impl_tailrec rs (packet_set_opt (packet_set_union P (to_packet_set Accept m)))  ((packet_set_union P  (packet_set_not (to_packet_set Accept m)))# PAs)" |
-  "collect_allow_compl_v2_impl_tailrec ((Rule m Drop)#rs) P PAs = collect_allow_compl_v2_impl_tailrec rs (packet_set_opt (packet_set_union P (to_packet_set Drop m))) PAs"
+fun collect_allow_compl_impl_tailrec :: "'a rule list \<Rightarrow> 'a packet_set \<Rightarrow> 'a packet_set list \<Rightarrow> 'a packet_set list" where
+  "collect_allow_compl_impl_tailrec [] P PAs = PAs" |
+  "collect_allow_compl_impl_tailrec ((Rule m Accept)#rs) P PAs =
+     collect_allow_compl_impl_tailrec rs (packet_set_opt (packet_set_union P (to_packet_set Accept m)))  ((packet_set_union P  (packet_set_not (to_packet_set Accept m)))# PAs)" |
+  "collect_allow_compl_impl_tailrec ((Rule m Drop)#rs) P PAs = collect_allow_compl_impl_tailrec rs (packet_set_opt (packet_set_union P (to_packet_set Drop m))) PAs"
 
 
-lemma collect_allow_compl_v2_impl_tailrec_helper: "simple_ruleset rs \<Longrightarrow> 
-  (packet_set_to_set \<gamma> (collect_allow_compl_v2_impl rs P)) \<inter> (\<Inter> set (map (packet_set_to_set \<gamma>) PAs)) =
-  (\<Inter> set (map (packet_set_to_set \<gamma>) (collect_allow_compl_v2_impl_tailrec rs P PAs)))"
-proof(induction rs P arbitrary: PAs P rule: collect_allow_compl_v2_impl.induct)
+lemma collect_allow_compl_impl_tailrec_helper: "simple_ruleset rs \<Longrightarrow> 
+  (packet_set_to_set \<gamma> (collect_allow_compl_impl rs P)) \<inter> (\<Inter> set (map (packet_set_to_set \<gamma>) PAs)) =
+  (\<Inter> set (map (packet_set_to_set \<gamma>) (collect_allow_compl_impl_tailrec rs P PAs)))"
+proof(induction rs P arbitrary: PAs P rule: collect_allow_compl_impl.induct)
   case (2 m rs)
-    from 2 have IH: "(\<And>P PAs. packet_set_to_set \<gamma> (collect_allow_compl_v2_impl rs P) \<inter> (\<Inter>x\<in>set PAs. packet_set_to_set \<gamma> x) =
-                       (\<Inter>x\<in>set (collect_allow_compl_v2_impl_tailrec rs P PAs). packet_set_to_set \<gamma> x))"
+    from 2 have IH: "(\<And>P PAs. packet_set_to_set \<gamma> (collect_allow_compl_impl rs P) \<inter> (\<Inter>x\<in>set PAs. packet_set_to_set \<gamma> x) =
+                       (\<Inter>x\<in>set (collect_allow_compl_impl_tailrec rs P PAs). packet_set_to_set \<gamma> x))"
     by(simp add: simple_ruleset_def)
     from IH[where P="(packet_set_opt (packet_set_union P (to_packet_set Accept m)))" and PAs="(packet_set_union P (packet_set_not (to_packet_set Accept m)) # PAs)"] have
       "(packet_set_to_set \<gamma> P \<union> {p. \<not> matches \<gamma> m Accept p}) \<inter> 
-       packet_set_to_set \<gamma> (collect_allow_compl_v2_impl rs (packet_set_opt (packet_set_union P (to_packet_set Accept m)))) \<inter>
+       packet_set_to_set \<gamma> (collect_allow_compl_impl rs (packet_set_opt (packet_set_union P (to_packet_set Accept m)))) \<inter>
        (\<Inter>x\<in>set PAs. packet_set_to_set \<gamma> x) =
        (\<Inter>x\<in>set
-        (collect_allow_compl_v2_impl_tailrec rs (packet_set_opt (packet_set_union P (to_packet_set Accept m))) (packet_set_union P (packet_set_not (to_packet_set Accept m)) # PAs)).
+        (collect_allow_compl_impl_tailrec rs (packet_set_opt (packet_set_union P (to_packet_set Accept m))) (packet_set_union P (packet_set_not (to_packet_set Accept m)) # PAs)).
           packet_set_to_set \<gamma> x)"
         apply(simp add: packet_set_union_correct packet_set_not_correct to_packet_set_set) by blast
     thus ?case
@@ -727,21 +788,21 @@ qed(simp_all add: simple_ruleset_def packet_set_union_correct packet_set_opt_cor
       to_packet_set_set set_helper1 packet_set_constrain_not_correct packet_set_UNIV packet_set_Empty_def)
 
 
-lemma collect_allow_compl_v2_impl_tailrec_correct: "simple_ruleset rs \<Longrightarrow> 
-  (packet_set_to_set \<gamma> (collect_allow_compl_v2_impl rs P)) = (\<Inter>x\<in>set (collect_allow_compl_v2_impl_tailrec rs P []). packet_set_to_set \<gamma> x)"
-using collect_allow_compl_v2_impl_tailrec_helper[where PAs="[]", simplified]
+lemma collect_allow_compl_impl_tailrec_correct: "simple_ruleset rs \<Longrightarrow> 
+  (packet_set_to_set \<gamma> (collect_allow_compl_impl rs P)) = (\<Inter>x\<in>set (collect_allow_compl_impl_tailrec rs P []). packet_set_to_set \<gamma> x)"
+using collect_allow_compl_impl_tailrec_helper[where PAs="[]", simplified]
 by metis
 
 
 definition allow_set_not_inter :: "'a rule list \<Rightarrow> 'a packet_set list" where
-  "allow_set_not_inter rs \<equiv> collect_allow_compl_v2_impl_tailrec rs packet_set_Empty []"
+  "allow_set_not_inter rs \<equiv> collect_allow_compl_impl_tailrec rs packet_set_Empty []"
 
 text{*Intersecting over the result of @{const allow_set_not_inter} and inverting is the list of all allowed packets*}
 lemma allow_set_not_inter: "simple_ruleset rs \<Longrightarrow> 
   - (\<Inter>x\<in>set (allow_set_not_inter rs). packet_set_to_set \<gamma> x) = {p. approximating_bigstep_fun \<gamma> p rs Undecided = Decision FinalAllow}"
   unfolding allow_set_not_inter_def
-  apply(simp add: collect_allow_compl_v2_impl_tailrec_correct[symmetric])
-  apply(simp add:collect_allow_compl_v2_impl)
+  apply(simp add: collect_allow_compl_impl_tailrec_correct[symmetric])
+  apply(simp add:collect_allow_compl_impl)
   apply(simp add: packet_set_Empty)
   using collect_allow_sound_complete by fast 
 
